teleport and ghz examples

MoreExamples.v
@@ -1,105 +1,54 @@
-(* Example 11: Remove XOR *)
+Require Import Typing.
 
-(** * Own examples *)
+(** * Superdense coding *)
 
-(** * Proofs about derived unitaries *)
+Definition bell00 : prog := H' 2; CNOT 2 3.
 
-Lemma X_X1 : @h_eval 1 (X 0) [XX] = [XX].
-Proof. reflexivity. Qed.
-Lemma X_Z1 : @h_eval 1 (X 0) [ZZ] = [-1 * ZZ].
-Proof. reflexivity. Qed.
-Lemma Y_X1 : @h_eval 1 (Y 0) [XX] = [-1 * XX].
-Proof. reflexivity. Qed.
-Lemma Y_Z1 : @h_eval 1 (Y 0) [ZZ] = [-1 * ZZ].
-Proof. reflexivity. Qed.
-Lemma Z_X1 : @h_eval 1 (Z 0) [XX] = [-1 * XX].
-Proof. reflexivity. Qed.
-Lemma Z_Z1 : @h_eval 1 (Z 0) [ZZ] = [ZZ].
-Proof. reflexivity. Qed.
+Definition encode : prog := CZ 0 2; CNOT 1 2.
 
-Lemma CZ_X1 : @h_eval 2 (CZ 0 1) [XX,II] = [XX,ZZ].
-Proof. reflexivity. Qed.
-Lemma CZ_Z1 : @h_eval 2 (CZ 0 1) [ZZ,II] = [ZZ,II].
-Proof. reflexivity. Qed.
-Lemma CZ_X2 : @h_eval 2 (CZ 0 1) [II,XX] = [ZZ,XX].
-Proof. reflexivity. Qed.
-Lemma CZ_Z2 : @h_eval 2 (CZ 0 1) [II,ZZ] = [II,ZZ].
-Proof. reflexivity. Qed.
-
-(* Superdense coding *)
-
-Definition bell00 : prog 4 :=
-  H 2;
-  CNOT 2 3.
-
-Definition encode : prog 4 :=
-    CZ 0 2; CNOT 1 2.
-
-Definition decode : prog 4 :=
-  CNOT 2 3;
-  H 2.
+Definition decode : prog := CNOT 2 3; H' 2.
 
 Definition superdense := bell00 ; encode; decode.
 
-Compute (h_eval superdense [ZZ,ZZ,ZZ,ZZ]). (* I, I, Z, Z *)
-Compute (h_eval superdense [II,ZZ,ZZ,ZZ]). (* Z, I, Z, Z *)
-Compute (h_eval superdense [ZZ,II,ZZ,ZZ]). (* I, Z, Z, Z *)
-Compute (h_eval superdense [II,II,ZZ,ZZ]). (* Z, Z, Z, Z *)
-Compute (h_eval superdense [ZZ,ZZ,ZZ,II]). (* I, Z, Z, I *)
-Compute (h_eval superdense [ZZ,ZZ,II,ZZ]). (* Z, I, I, Z *)
+Lemma superdenseTypesQPL : superdense :: (Z ⊗ Z ⊗ Z ⊗ Z → I ⊗ I ⊗ Z ⊗ Z).
+Proof. type_check_base. Qed.
 
-Compute (h_eval superdense [ZZ,II,II,II]). (* Z, I, I, I *)
-Compute (h_eval superdense [II,ZZ,II,II]). (* I, Z, I, I *)
-Compute (h_eval superdense [II,II,ZZ,II]). (* Z, I, Z, I *)
-Compute (h_eval superdense [II,II,II,ZZ]). (* I, Z, I, Z *)
+Lemma superdenseTypes : superdense :: (Z ⊗ I ⊗ I ⊗ I → Z ⊗ I ⊗ I ⊗ I) ∩
+                                     (I ⊗ Z ⊗ I ⊗ I → I ⊗ Z ⊗ I ⊗ I) ∩
+                                     (I ⊗ I ⊗ Z ⊗ I → Z ⊗ I ⊗ Z ⊗ I) ∩
+                                     (I ⊗ I ⊗ I ⊗ Z → I ⊗ Z ⊗ I ⊗ Z).
+Proof. type_check_base. Qed.
 
 
-Lemma superdense_ZZ : h_eval superdense [ZZ,ZZ,ZZ,ZZ] = [II,II,ZZ,ZZ].
-Proof. reflexivity. Qed.
 
-(* GHZ state *)
+(** * GHZ state *)
 
-Compute (h_eval (CNOT 0 1) [XX*ZZ, ZZ]). (* X, XZ *)
+Definition GHZ3 : prog := H' 0; CNOT 0 1; CNOT 1 2.
 
-Definition GHZ3 : prog :=
-  H 0;
-  CNOT 0 1;
-  CNOT 1 2.
+Lemma GHZ3Types : GHZ3 :: (Z ⊗ I ⊗ I → X ⊗ X ⊗ X) ∩
+                         (I ⊗ Z ⊗ I → Z ⊗ Z ⊗ I) ∩
+                         (I ⊗ I ⊗ Z → I ⊗ Z ⊗ Z).
+Proof. type_check_base. Qed.
 
-Compute (h_eval GHZ3 [ZZ,ZZ,ZZ]). (* XZ, X, XZ *)
-
-Compute (h_eval GHZ3 [XX,II,II]). (* Z, I, I *)
-Compute (h_eval GHZ3 [II,XX,II]). (* I, X, X *)
-Compute (h_eval GHZ3 [II,II,XX]). (* I, I, X *)
-Compute (h_eval GHZ3 [II,ZZ,ZZ]). (* Z, I, Z *)
-Compute (h_eval GHZ3 [XX,ZZ,ZZ]). (* I, I, Z *)
-Compute (h_eval GHZ3 [XX,II,ZZ]). (* Z, Z, Z *)
-Compute (h_eval GHZ3 [XX,ZZ,II]). (* I, Z, I *)
-
-Compute (h_eval GHZ3 [ZZ,II,II]). (* X, X, X *)
-Compute (h_eval GHZ3 [II,ZZ,II]). (* Z, Z, I *)
-Compute (h_eval GHZ3 [II,II,ZZ]). (* I, Z, Z *)
-
-
-Compute (h_eval (CNOT 1 2; CNOT 0 1) [XX*ZZ,XX,XX*ZZ]). (* X, Z, Z ??? *)
-Compute (h_eval (CNOT 0 1; CNOT 1 2) [XX*ZZ,XX,XX*ZZ]). (* X, Z, Z ??? *)
+(* Note: The second and third cases do contain GHZ as eigenvectors, as we'd expect.
+   But didn't we say these are separable? *)
 
 (** Honda motivating example *)
 
-Definition SEP0 := GHZ3 ; CNOT 0 1; CNOT 0 2.
+Definition SEP0 := GHZ3; CNOT 0 1; CNOT 0 2.
 
-Compute (h_eval SEP0 [ZZ,II,II]). (* X, I, I *)
-Compute (h_eval SEP0 [II,ZZ,II]). (* I, Z, I *)
-Compute (h_eval SEP0 [II,II,ZZ]). (* I, Z, Z *) (* becomes I, I, Z *)
+Lemma SEP0Types : SEP0 :: (Z ⊗ I ⊗ I → X ⊗ I ⊗ I) ∩
+                         (I ⊗ Z ⊗ I → I ⊗ Z ⊗ I) ∩
+                         (I ⊗ I ⊗ Z → I ⊗ Z ⊗ Z).
+Proof. type_check_base. Qed.
 
 (* Result : X × Z × Z *)
 
 (** Unentangling one qubit *)
 
-Compute (h_eval (GHZ3;CNOT 1 2) [ZZ,II,II]). (* X, X, I *)
-Compute (h_eval (GHZ3;CNOT 1 2) [II,ZZ,II]). (* Z, Z, I *)
-Compute (h_eval (GHZ3;CNOT 1 2) [II,II,ZZ]). (* I, I, Z *)
+Definition PSEP := GHZ3; CNOT 1 2.
 
-Compute (h_eval (GHZ3;CNOT 2 1) [ZZ,II,II]). (* X, I, X *)
-Compute (h_eval (GHZ3;CNOT 2 1) [II,ZZ,II]). (* Z, Z, Z *) (* becomes Z, I, Z *)
-Compute (h_eval (GHZ3;CNOT 2 1) [II,II,ZZ]). (* I, Z, I *)
+Lemma PSEPTypes : PSEP :: (Z ⊗ I ⊗ I → X ⊗ X ⊗ I) ∩
+                         (I ⊗ Z ⊗ I → Z ⊗ Z ⊗ I) ∩
+                         (I ⊗ I ⊗ Z → I ⊗ I ⊗ Z).
+Proof. type_check_base. Qed.
